code/ecdsa/Hacl.Impl.EC.PointAdd.fsti
@@ -19,15 +19,15 @@ let fromDomain #c = fromDomain_ #c #DH
 inline_for_extraction noextract
 val point_add: #c: curve -> p: point c -> q: point c -> result: point c 
   -> tempBuffer: lbuffer uint64 (size 17 *! getCoordinateLenU64 c) -> 
-  Stack unit (requires fun h -> 
+  Stack unit 
+  (requires fun h -> 
     live h p /\ live h q /\ live h result /\ live h tempBuffer /\ 
     eq_or_disjoint q result /\ disjoint p q /\ disjoint p tempBuffer /\ 
     disjoint q tempBuffer /\ disjoint p result /\ disjoint result tempBuffer /\  
     point_eval c h p /\ point_eval c h q)
-  (ensures fun h0 _ h1 -> modifies (loc tempBuffer |+| loc result) h0 h1 /\ point_eval c h1 result /\
-    fromDomainPoint #c #DH (point_as_nat c h1 result) == _point_add #c (fromDomainPoint #c #DH (point_as_nat c h0 p)) (fromDomainPoint #c #DH (point_as_nat c h0 q)))
+  (ensures fun h0 _ h1 -> modifies (loc tempBuffer |+| loc result) h0 h1)
 
-
+  
 inline_for_extraction noextract
 val point_add_out: #c: curve -> p: point c -> q: point c -> result: point c -> 
   Stack unit (requires fun h -> live h p /\ live h q /\ live h result /\ 
