code/ecdsa/Hacl.Impl.EC.PointAddC.fsti
@@ -19,19 +19,8 @@ open FStar.Mul
 inline_for_extraction
 val point_add_c: #c: curve -> p: point c -> q: point c -> result: point c 
   -> tempBuffer: lbuffer uint64 (size 17 *! getCoordinateLenU64 c) -> 
-   Stack unit (requires fun h -> live h p /\ live h q /\ live h result /\ live h tempBuffer /\ 
-     eq_or_disjoint q result /\ disjoint p q /\ disjoint p tempBuffer /\ 
-     disjoint q tempBuffer /\ disjoint p result /\ disjoint result tempBuffer /\ 
-     point_eval c h p /\ point_eval c h q /\ ~ (isPointAtInfinity (point_as_nat c h p)) /\ 
-     ~ (isPointAtInfinity (point_as_nat c h q)))
-   (ensures fun h0 _ h1 -> modifies (loc tempBuffer |+| loc result) h0 h1 /\ point_eval c h1 result /\ (
-     let pD = fromDomainPoint #c #DH (point_as_nat c h0 p) in 
-     let qD = fromDomainPoint #c #DH (point_as_nat c h0 q) in 
-(*      if pointEqual #c pD qD then 
-       fromDomainPoint #c #DH (point_as_nat c h1 result) == _point_double_nist #c pD
-     else
-       fromDomainPoint #c #DH (point_as_nat c h1 result) == _point_add #c pD qD /\ *)
-     fromDomainPoint #c #DH (point_as_nat c h1 result) == pointAdd #c pD qD))
+   Stack unit (requires fun h -> True)
+   (ensures fun h0 _ h1 -> modifies (loc tempBuffer |+| loc result) h0 h1)
 
 
 
@@ -39,8 +28,8 @@ inline_for_extraction noextract
 val point_add_c_out: #c: curve -> p: point c -> q: point c -> result: point c ->
   Stack unit (requires fun h -> live h p /\ live h q /\ live h result /\ 
     eq_or_disjoint q result /\ disjoint p q /\ disjoint p result /\
-     point_eval c h p /\ point_eval c h q /\ ~ (isPointAtInfinity (point_as_nat c h p)) /\ 
-     ~ (isPointAtInfinity (point_as_nat c h q)))
+     point_eval c h p /\ point_eval c h q /\ ~ (isPointAtInfinity #Jacobian (point_as_nat c h p)) /\ 
+     ~ (isPointAtInfinity #Jacobian (point_as_nat c h q)))
    (ensures fun h0 _ h1 -> modifies (loc result) h0 h1 /\ point_eval c h1 result /\ (
      let pD = fromDomainPoint #c #DH (point_as_nat c h0 p) in 
      let qD = fromDomainPoint #c #DH (point_as_nat c h0 q) in 
